Working on alpha term_rep proof
Defined term_rep
Proved all term cases except Tmatch
Tmatch mostly done
Need to know all pattern free vars in resulting map
Requires some more detailed proofs about patterns with typing (for disj)
In middle of these proofs

proofs/core/Alpha.v
@@ -993,10 +993,758 @@ Proof.
         -- rewrite amap_set_lookup_same; reflexivity.
       * rewrite amap_set_lookup_diff by auto. (*from IH*) auto.
 Qed.
+
+(*Need separate lemma: if variable x is in m but is NOT in free vars of p, then it is still in res 
+  (with same binding, but probably dont need)
+  Again, will need typing for same reason
+  Then lift this to fold result with [big_union]
+  Then use this result to show that after 1 step in (bc in free vars), then still in after res
+  START here*)
+
+(*One more result we need (TODO: move above): every pattern free var is in the corresponding map after*)
+Lemma alpha_equiv_p_all_fv {p1 p2: pattern} {m res: amap vsymbol vsymbol * amap vsymbol vsymbol} {ty1 ty2}
+  (Hty1: pattern_has_type gamma p1 ty1) (*For disjoint free vars in constr*)
+  (Hty2: pattern_has_type gamma p2 ty2)
+  (Halpha: alpha_equiv_p m p1 p2 = Some res) x:
+  (forall (Hmem: aset_mem x (pat_fv p1)), amap_mem x (fst res)) /\
+  (forall (Hmem: aset_mem x (pat_fv p2)), amap_mem x (snd res)).
+Proof.
+  generalize dependent res. generalize dependent m. generalize dependent ty2.
+  generalize dependent ty1. revert p2.
+  induction p1 as [v1 | f1 tys1 ps1 IH | | p1 q1 IH1 IH2 | p1 v1 IH].
+  - intros [v2| | | |]; intros; inversion Halpha; subst; auto; clear Halpha.
+    simpl. simpl_set.
+    apply alpha_p_var_some in H0. subst; simpl in *.
+    split; intros; subst;
+    rewrite amap_mem_spec, amap_set_lookup_same; reflexivity.
+  - intros [| f2 tys2 ps2 | | |] ty1 Hty1 ty2 Hty2 m res Halpha; try discriminate. simpl in Halpha.
+    destruct (funsym_eq_dec f1 f2); subst; [|discriminate].
+    destruct (Nat.eqb_spec (length ps1) (length ps2)) as [Hlen | Hlen]; [|discriminate].
+    destruct (list_eq_dec _ _); subst ;[|discriminate].
+    simpl in *.
+    unfold option_collapse in *.
+    destruct (fold_left2 _ _ _ _) as [[r1|]|] eqn : Hfold; [|discriminate | discriminate].
+    (*Need typing and disjoint results but that is it*)
+    assert (Hdisj1:=pat_constr_disj_map Hty1).
+    assert (Hdisj2:=pat_constr_disj_map Hty2).
+    assert (Hlensubst: length (ty_subst_list (s_params f2) tys2 (s_args f2)) = length ps1). {
+      inversion Hty1; subst; unfold ty_subst_list. solve_len.
+    }
+    assert (Htys1: Forall2 (pattern_has_type gamma) ps1 (ty_subst_list (s_params f2) tys2 (s_args f2))).
+    { inversion Hty1; subst. rewrite Forall2_combine, Forall_forall; split; auto. }
+    assert (Htys2: Forall2 (pattern_has_type gamma) ps2 (ty_subst_list (s_params f2) tys2 (s_args f2))).
+    { inversion Hty2; subst. rewrite Forall2_combine, Forall_forall; split; auto; lia. }
+    clear Hty1 Hty2.
+    generalize dependent (ty_subst_list (s_params f2) tys2 (s_args f2)).
+    (*Now nested induction*)
+    inversion Halpha; subst; clear Halpha.
+    generalize dependent res. generalize dependent m. generalize dependent ps2.
+    induction ps1 as [| p1 ps1 IHps]; intros [| p2 ps2] Hlen Hdisj2; try discriminate; simpl; 
+    intros m res Hfold tys Htyslen Htys1 Htys2.
+    { (*empty case is easy*) simpl_set. split; intros; simpl_set. }
+    rewrite !aset_big_union_cons. simpl_set_small.
+    (*Get assumptions for IH*) destruct tys as [| tyh tys1]; [inversion Htys1|]. simpl in Hlen, Htyslen.
+    assert (Hdisj1':=disj_map_cons_impl Hdisj1).
+    assert (Hdisj2':=disj_map_cons_impl Hdisj2).
+    inversion Htys1; inversion Htys2; subst.
+    inversion IH; subst.
+    (*Annoying part comes from fold*)
+    split; intros [Hmemx | Hmemx].
+    + eapply H1; eauto.
+    disj_map_cons_impl
+    (*Get disjoint assumptions correct*)
+    Search disj_map' cons.
+    rewrite aset_big_union_cons in Hmem. simpl_set_small. 
+    inversion IH; subst.
+    assert (Halpha:=Hfold); apply fold_left2_bind_base_some in Halpha.
+    destruct Halpha as [r1 Halpha].
+    rewrite Halpha in Hfold.
+    destruct Hmem as [Hhd | Hmem].
+    (*TODO: need some disj assumptions, makes sense, need to prove we don't override things.
+      Here, assume typing and use disj assumption*)
+    + eapply H1; eauto.
+
+
+(*Get single equiv*)
+
+      specialize (IHps H2 ps2 (ltac:(simpl in Hlen; lia)) _ _ Hfold).
+      intros Hmem. simpl_set_small.
+      apply IHps in Hmem; destruct Hmem; auto.
+      * eapply H1 in H; eauto. destruct_all; auto.
+      * destruct_all; auto.
+  - intros [| | | |]; intros; inversion Halpha; subst; auto.
+  - (*Por case*)
+    intros [| | | p2 q2 |] m res Halpha; inversion Halpha; subst; clear Halpha.
+    apply option_bind_some in H0. destruct H0 as [r1 [Halpha Horcmp]].
+    (*Easy: we don't change map in [or_cmp]*)
+    destruct (or_cmp (fst r1) (snd r1) q1 q2); [|discriminate].
+    inversion Horcmp; subst. intros Hlookup. apply IH1 in Halpha; auto.
+    simpl. simpl_set.
+    destruct_all; auto.
+  - (*Pbind*)
+    intros [| | | | p2 v2] m res Halpha; inversion Halpha; subst; clear Halpha.
+    apply option_bind_some in H0. destruct H0 as [r1 [Halpha Hvar]].
+    intros Hlookup.
+    simpl. simpl_set. 
+    apply alpha_p_var_some in Hvar. subst; simpl in *.
+    destruct (vsymbol_eq_dec x v1); subst; auto.
+    + rewrite amap_set_lookup_same in Hlookup by auto. inversion Hlookup; subst; auto.
+    + rewrite amap_set_lookup_diff in Hlookup by auto.
+      eapply IH with (p2:=p2) in Hlookup; eauto.
+      destruct_all; auto.
+Qed.
+
+(*Corollaries for empty maps*)
+
+(*TODO: move*)
+Lemma bij_empty: bij_map amap_empty amap_empty.
+Proof.
+  unfold bij_map. intros x y. rewrite !amap_empty_get. split; discriminate.
+Qed.
+
+Corollary a_equiv_p_bij {p1 p2: pattern} {res}:
+  a_equiv_p p1 p2 = Some res ->
+  bij_map (fst res) (snd res).
+Proof.
+  intros Halpha.
+  eapply alpha_equiv_p_bij; eauto.
+  apply bij_empty.
+Qed.
+
+(*Idea: for every binding (x, y) in first map, we know that x in fv of p1 and y in fv in p2*)
+Corollary a_equiv_p_vars {p1 p2: pattern} {res}
+  (Halpha: a_equiv_p p1 p2 = Some res) x y (Hmem: amap_lookup (fst res) x = Some y):
+  aset_mem x (pat_fv p1) /\ aset_mem y (pat_fv p2).
+Proof.
+  eapply alpha_equiv_p_vars in Hmem; eauto.
+  simpl in Hmem. rewrite amap_empty_get in Hmem. destruct_all; auto; discriminate.
+Qed.
+
+Corollary match_val_single_alpha_p_full {ty: vty} {p1 p2: pattern}
+  (Hty1: pattern_has_type gamma p1 ty)
+  (Hty2: pattern_has_type gamma p2 ty)
+  (d: domain (dom_aux pd) (v_subst vt ty))
+  {res}
+  (Halpha: a_equiv_p p1 p2 = Some res):
+  opt_related (fun s1 s2 =>
+    forall x y t,
+    amap_lookup (fst res) x = Some y ->
+    amap_lookup s1 x = Some t <-> amap_lookup s2 y = Some t)
+  (match_val_single gamma_valid pd pdf vt ty p1 Hty1 d)
+  (match_val_single gamma_valid pd pdf vt ty p2 Hty2 d).
+Proof.
+  apply match_val_single_alpha_p with (m:=(amap_empty, amap_empty)); auto.
+  - apply bij_empty. 
+  - eapply a_equiv_p_bij; eauto.
+Qed.
+
+
+  
+
+
      
 (*START
   Still need (for patterns): Typing, probably reflexivity, symmetry, etc - but TODO see
 *)
+
+(*Define alpha equivalence for terms and formulas - use 2 maps, but basically like
+  pattern [or_cmp] - we pass in correct maps*)
+
+(*This time, vars either map appropriately in map or equal (free vars *)
+Definition alpha_equiv_var (m1 m2: amap vsymbol vsymbol) (v1 v2: vsymbol) : bool :=
+  match amap_lookup m1 v1, amap_lookup m2 v2 with
+  | Some v3, Some v4 => vsymbol_eq_dec v2 v3 && vsymbol_eq_dec v1 v4
+  | None, None => vsymbol_eq_dec v1 v2
+  | _, _ => false (*None, None case should never happen*)
+  end.
+
+(*TODO: prove iff*)
+Lemma alpha_equiv_var_iff m1 m2 v1 v2:
+  alpha_equiv_var m1 m2 v1 v2 <-> (amap_lookup m1 v1 = Some v2 /\ amap_lookup m2 v2 = Some v1) \/
+    (amap_lookup m1 v1 = None /\ amap_lookup m2 v2 = None /\ v1 = v2).
+Proof.
+  unfold alpha_equiv_var. destruct (amap_lookup m1 v1) as [v3|];
+  destruct (amap_lookup m2 v2) as [v4|];
+  try solve[split; intros; destruct_all; discriminate].
+  - rewrite andb_true. split.
+    + intros [Heq1 Heq2]. vsym_eq v2 v3; vsym_eq v1 v4; discriminate.
+    + intros [[Heq1 Heq2] | [Heq _]]; try discriminate.
+      inversion Heq1; inversion Heq2; subst. vsym_eq v2 v2; vsym_eq v1 v1.
+  - vsym_eq v1 v2; simpl; split; try discriminate; auto.
+    intros; destruct_all; subst; try discriminate; contradiction.
+Qed.
+  
+
+
+(* Lemma or_cmp_vsym_iff m1 m2 v1 v2:
+  or_cmp_vsym m1 m2 v1 v2 <-> amap_lookup m1 v1 = Some v2 /\ amap_lookup m2 v2 = Some v1.
+Proof.
+  unfold or_cmp_vsym. destruct (amap_lookup m1 v1) as [v3|].
+  2: split; intros; destruct_all; discriminate.
+  destruct (amap_lookup m2 v2) as [v4|].
+  2: split; intros; destruct_all; discriminate.
+  destruct (vsymbol_eq_dec v2 v3); subst; simpl.
+  - destruct (vsymbol_eq_dec v1 v4); subst; simpl; auto.
+    + split; auto.
+    + split; try discriminate. intros [_ Hsome]; inversion Hsome; subst; contradiction.
+  - split; try discriminate. intros [Hsome _]; inversion Hsome; subst; contradiction.
+Qed. *)
+
+(* Definition add_binding (m1 m2: amap vsymbol vsymbol) (v1 v2: vsymbol) : amap *)
+
+Fixpoint alpha_equiv_t (m1 m2: amap vsymbol vsymbol) (t1 t2: term) : bool :=
+  match t1, t2 with
+  | Tconst c1, Tconst c2 =>
+    const_eq_dec c1 c2
+  | Tvar v1, Tvar v2 =>
+    alpha_equiv_var m1 m2 v1 v2
+  | Tfun f1 ty1 tm1, Tfun f2 ty2 tm2 =>
+    (funsym_eq_dec f1 f2) &&
+    (length tm1 =? length tm2) && 
+    (list_eq_dec vty_eq_dec ty1 ty2) &&
+    (all2 (fun t1 t2 => alpha_equiv_t m1 m2 t1 t2)) tm1 tm2
+  | Tlet tm1 x tm2, Tlet tm3 y tm4 =>
+    vty_eq_dec (snd x) (snd y) &&
+    alpha_equiv_t m1 m2 tm1 tm3 &&
+    (*Add new binding*) (*TODO: make sure we dont have situation like patterns*)
+    alpha_equiv_t (amap_set m1 x y) (amap_set m2 y x) tm2 tm4
+  | Tif f1 t1 t3, Tif f2 t2 t4 =>
+    alpha_equiv_f m1 m2 f1 f2 &&
+    alpha_equiv_t m1 m2 t1 t2 &&
+    alpha_equiv_t m1 m2 t3 t4
+  | Tmatch t1 ty1 ps1, Tmatch t2 ty2 ps2 =>
+    alpha_equiv_t m1 m2 t1 t2 &&
+    (length ps1 =? length ps2) &&
+    (vty_eq_dec ty1 ty2) &&
+    (*Use map from pattern, merge with existing maps*)
+    all2 (fun (x1 x2: pattern * term) =>
+      match (a_equiv_p (fst x1) (fst x2)) with
+      | Some (pm1, pm2) => alpha_equiv_t 
+          (amap_union (fun x _ => Some x) pm1 m1) (amap_union (fun x _ => Some x) pm2 m2) (snd x1) (snd x2)
+      | None => false
+      end) ps1 ps2
+      (* alpha_equiv_p (combine (pat_fv (fst x1)) (pat_fv (fst x2)))
+        (fst x1) (fst x2) &&
+      alpha_equiv_t (add_vals (pat_fv (fst x1)) (pat_fv (fst x2)) vars)
+        (snd x1) (snd x2)) ps1 ps2 *)
+  | Teps f1 x, Teps f2 y => 
+    vty_eq_dec (snd x) (snd y) &&
+    alpha_equiv_f (amap_set m1 x y) (amap_set m2 y x) f1 f2
+  | _, _ => false
+  end
+with alpha_equiv_f (m1 m2: amap vsymbol vsymbol) (f1 f2: formula) {struct f1} : bool :=
+  match f1, f2 with
+  | Fpred p1 ty1 tm1, Fpred p2 ty2 tm2 =>
+    (predsym_eq_dec p1 p2) &&
+    (length tm1 =? length tm2) && 
+    (list_eq_dec vty_eq_dec ty1 ty2) &&
+    (all2 (fun t1 t2 => alpha_equiv_t m1 m2 t1 t2)) tm1 tm2
+  | Fquant q1 x f1, Fquant q2 y f2 =>
+    quant_eq_dec q1 q2 &&
+    vty_eq_dec (snd x) (snd y) &&
+    alpha_equiv_f (amap_set m1 x y) (amap_set m2 y x) f1 f2
+  | Feq ty1 t1 t3, Feq ty2 t2 t4 =>
+    vty_eq_dec ty1 ty2 &&
+    alpha_equiv_t m1 m2 t1 t2 &&
+    alpha_equiv_t m1 m2 t3 t4
+  | Fbinop b1 f1 f3, Fbinop b2 f2 f4 =>
+    binop_eq_dec b1 b2 &&
+    alpha_equiv_f m1 m2 f1 f2 &&
+    alpha_equiv_f m1 m2 f3 f4
+  | Fnot f1, Fnot f2 =>
+    alpha_equiv_f m1 m2 f1 f2
+  | Ftrue, Ftrue => true
+  | Ffalse, Ffalse => true
+  | Flet t1 x f1, Flet t2 y f2 =>
+    vty_eq_dec (snd x) (snd y) &&
+    alpha_equiv_t m1 m2 t1 t2 &&
+    alpha_equiv_f (amap_set m1 x y) (amap_set m2 y x) f1 f2
+  | Fif f1 f3 f5, Fif f2 f4 f6 =>
+    alpha_equiv_f m1 m2 f1 f2 &&
+    alpha_equiv_f m1 m2 f3 f4 &&
+    alpha_equiv_f m1 m2 f5 f6
+  | Fmatch t1 ty1 ps1, Fmatch t2 ty2 ps2 =>
+    alpha_equiv_t m1 m2 t1 t2 &&
+    (length ps1 =? length ps2) &&
+    (vty_eq_dec ty1 ty2) &&
+    all2 (fun (x1 x2: pattern * formula) =>
+      match (a_equiv_p (fst x1) (fst x2)) with
+      | Some (pm1, pm2) => alpha_equiv_f 
+          (amap_union (fun x _ => Some x) pm1 m1) (amap_union (fun x _ => Some x) pm2 m2) (snd x1) (snd x2)
+      | None => false
+      end) ps1 ps2
+  | _, _ => false
+  end.
+
+(*Full alpha equivalence: when there are no vars in the
+  context*)
+Definition a_equiv_t: term -> term -> bool :=
+  alpha_equiv_t amap_empty amap_empty.
+Definition a_equiv_f: formula -> formula -> bool :=
+  alpha_equiv_f amap_empty amap_empty.
+
+(*TODO: move*)
+Lemma amap_set_lookup_iff {A B: Type} `{countable.Countable A} (m: amap A B) (x1 x2 : A) (y1 y2: B):
+  amap_lookup (amap_set m x1 y1) x2 = Some y2 <-> (x1 = x2 /\ y1 = y2) \/ (x1 <> x2 /\ amap_lookup m x2 = Some y2).
+Proof.
+  destruct (EqDecision0 x1 x2); subst.
+  - rewrite amap_set_lookup_same. split.
+    + intros Hsome; inversion Hsome; auto.
+    + intros; destruct_all; subst; auto. contradiction.
+  - rewrite amap_set_lookup_diff by auto. 
+    split; intros; destruct_all; subst; auto. contradiction.
+Qed. 
+
+Lemma amap_set_lookup_none_iff {A B: Type} `{countable.Countable A} (m: amap A B) (x1 x2 : A) (y1: B):
+  amap_lookup (amap_set m x1 y1) x2 = None <-> (x1 <> x2 /\ amap_lookup m x2 = None).
+Proof.
+  destruct (EqDecision0 x1 x2); subst.
+  - rewrite amap_set_lookup_same. split; try discriminate. intros; destruct_all; contradiction.
+  - rewrite amap_set_lookup_diff by auto. split; intros; destruct_all; auto.
+Qed. 
+(*And prove semantics - TODO organize contexts better*)
+
+ (*Idea: variables mapped in both have same valuations (up to casting)
+    and variables in neither map also same (unaffected).
+    The ambiguous case is when a variable is mapped in one but not another.
+    We don't actually need this case, since if we look up such a variable, the terms are NOT
+    alpha equivalent*)
+Lemma alpha_equiv_rep (t1: term) (f1: formula) :
+  (forall (t2: term) (m1 m2: amap vsymbol vsymbol)
+  (v1 v2: val_vars pd vt) (ty: vty)
+  (Hty1: term_has_type gamma t1 ty)
+  (Hty2: term_has_type gamma t2 ty)
+  (Heq: alpha_equiv_t m1 m2 t1 t2)
+  (Hvals: forall x y (Heq: snd x = snd y),
+    (*This is matched in BOTH maps*)
+    amap_lookup m1 x = Some y ->
+    amap_lookup m2 y = Some x ->
+    v1 x = (dom_cast _ (f_equal _ (eq_sym Heq)) (v2 y)))
+  (Hvals2: forall x,
+    amap_lookup m1 x = None ->
+    amap_lookup m2 x = None ->
+    v1 x = v2 x),
+  term_rep v1 t1 ty Hty1 = term_rep v2 t2 ty Hty2) /\
+  (forall (f2: formula) (m1 m2: amap vsymbol vsymbol) 
+  (v1 v2: val_vars pd vt)
+  (Hval1: formula_typed gamma f1)
+  (Hval2: formula_typed gamma f2)
+  (Heq: alpha_equiv_f m1 m2 f1 f2)
+  (Hvals1: forall x y (Heq: snd x = snd y),
+    amap_lookup m1 x = Some y ->
+    amap_lookup m2 y = Some x ->
+    v1 x = (dom_cast _ (f_equal _ (eq_sym Heq)) (v2 y)))
+  (Hvals2: forall x,
+    amap_lookup m1 x = None ->
+    amap_lookup m2 x = None ->
+    v1 x = v2 x),
+  formula_rep v1 f1 Hval1 = formula_rep v2 f2 Hval2).
+Proof.
+  revert t1 f1. apply term_formula_ind; simpl; intros;auto.
+  - (*Tconst*) destruct t2; try discriminate. destruct (const_eq_dec _ _); subst; [|discriminate].
+    erewrite term_rep_irrel. apply tm_change_vv; simpl. intros; simpl_set.
+  - (*Tvar*) destruct t2 as [| x2 | | | | |]; try discriminate. rename v into x1.
+    simpl_rep_full. unfold var_to_dom.
+    (*Use [alpha_equiv_var]*)
+    rewrite alpha_equiv_var_iff in Heq.
+    destruct Heq as [[Hlook1 Hlook2] | [Hlook1 [Hlook2 Heq]]].
+    + assert (Heq: snd x1 = snd x2). { inversion Hty1; inversion Hty2; subst; auto. } 
+      rewrite Hvals with (Heq:=Heq) by auto.
+      rewrite !dom_cast_compose. apply dom_cast_eq.
+    + subst. rewrite Hvals2 by auto. apply dom_cast_eq.
+  - (*Tfun*)
+    destruct t2 as [| | f2 tys2 tms2 | | | |] ; try discriminate.
+    rename l into tys1; rename l1 into tms1.
+    destruct (funsym_eq_dec _ _); subst; [|discriminate].
+    destruct (Nat.eqb_spec (length tms1) (length tms2)) as [Hlen|]; [|discriminate].
+    destruct (list_eq_dec _ _ _); subst; [|discriminate].
+    simpl in Heq.
+    simpl_rep_full.
+    (*Deal with casting*)
+    f_equal; [apply UIP_dec; apply vty_eq_dec |].
+    f_equal; [apply UIP_dec; apply sort_eq_dec |].
+    f_equal.
+    (*Now prove that arg_lists equivalent*)
+    apply get_arg_list_ext; auto.
+    rewrite all2_forall with(d1:=tm_d)(d2:=tm_d) in Heq; auto.
+    rewrite Forall_forall in H.
+    intros i Hi ty' Hty' Hty''. 
+    apply H with(m1:=m1)(m2:=m2); auto.
+    apply nth_In; auto.
+  - (*Tlet*)
+    destruct t2 as [| | | tm3 x2 tm4 | | |]; try discriminate.
+    rename v into x1.
+    simpl_rep_full.
+    destruct (vty_eq_dec _ _) as [Htyeq|]; [|discriminate].
+    simpl in Heq. rewrite andb_true in Heq. destruct Heq as [Halpha1 Halpha2].
+    eapply H0; eauto.
+    + (*TODO: separate lemma*) intros x y Heq Hlookup1 Hlookup2.
+      rewrite amap_set_lookup_iff in Hlookup1, Hlookup2.
+      destruct Hlookup1 as [[Hxeq Hyeq] | [Hneq Hlookup1]];
+      destruct Hlookup2 as [[Hxeq2 Hyeq2] | [Hneq2 Hlookup2]]; subst; try contradiction.
+      * unfold substi. vsym_eq x x. vsym_eq y y.
+        (*Now use first IH*)
+        assert (e = eq_refl) by (apply UIP_dec, vsymbol_eq_dec).
+        assert (e0 = eq_refl) by (apply UIP_dec, vsymbol_eq_dec).
+        subst. simpl.
+        (*Remove final cast*)
+        destruct x as [n1 ty1]; destruct y as [n2 ty2]; simpl in *; subst.
+        assert (Heq = eq_refl) by (apply UIP_dec, vty_eq_dec). subst; unfold dom_cast; simpl.
+        eapply H; eauto.
+      * (*2nd case, easy*)
+        unfold substi. vsym_eq x x1. vsym_eq y x2.
+    + (*None case*)
+      intros x Hnone1 Hnone2.
+      rewrite amap_set_lookup_none_iff in Hnone1, Hnone2.
+      destruct Hnone1 as [Hneq1 Hnone1]; destruct Hnone2 as [Hneq2 Hnone2].
+      unfold substi. vsym_eq x x1. vsym_eq x x2.
+  - (*Tif*)
+    destruct t0 as [| | | | f2 t3 t4 | |]; try discriminate.
+    bool_hyps. simpl_rep_full.
+    erewrite (H f2), (H0 t3), (H1 t4); try reflexivity; eauto.
+  - (*Tmatch*)
+    destruct t2 as [| | | | | tm2 ty2 ps2 |]; try discriminate.
+    rename tm into tm1; rename v into ty1; rename ps into ps1.
+    destruct (alpha_equiv_t m1 m2 tm1 tm2) eqn : Halpha; [|discriminate].
+    rewrite fold_is_true in Halpha. 
+    destruct (Nat.eqb_spec (length ps1) (length ps2)) as [Hlen |]; [|discriminate].
+    destruct (vty_eq_dec _ _); subst; [|discriminate].
+    simpl in Heq.
+    (*Need nested induction*)
+    rename H into Htm. rename H0 into Hps.
+    simpl_rep_full.
+    iter_match_gen Hty1 Htm1 Hpat1 Hty1.
+    iter_match_gen Hty2 Htm2 Hpat2 Hty2.
+    generalize dependent ps2.
+    induction ps1 as [|[p1 t1] ps1 IHps1]; simpl; intros [| [p2 t2] ps2]; intros; try discriminate; auto.
+    (*Only 1 interesting case*)
+    simpl.
+    (*First, simplify Htm*)
+    rewrite (Htm tm2 m1 m2 v1 v2 _ Hty1 Hty2) by auto.
+    (*Now use [match_val_single] result*)
+    rewrite all2_cons in Heq. simpl in Heq.
+    destruct (a_equiv_p p1 p2) as [[pm1 pm2] |] eqn: Halphap; [|discriminate].
+    rewrite andb_true in Heq. destruct Heq as [Halphat Hall].
+    pose proof (match_val_single_alpha_p_full (Forall_inv Hpat1) (Forall_inv Hpat2)
+      (term_rep v2 tm2 ty2 Hty2) Halphap) as Hopt. simpl in Hopt.
+    (*Now reason by cases; all but 2 trivial*)
+    destruct (match_val_single _ _ _ _ _ p1 _ _) as [a1|] eqn : Hmatch1;
+    destruct (match_val_single _ _ _ _ _ p2 _ _) as [a2|] eqn : Hmatch2;
+    simpl in Hopt; try contradiction; auto.
+    + (*Reason about [extend_val_with_list]*)
+      inversion Hps; subst. eapply H1; eauto.
+      * (*TODO: separate lemma?*)
+        intros x y Heq Hlookup1 Hlookup2.
+        rewrite amap_union_lookup in Hlookup1, Hlookup2.
+        (*NOTE: need to use free vars and bij information*)
+        assert (Hbij:=a_equiv_p_bij Halphap).
+        destruct (amap_lookup pm1 x) as [y1|] eqn : Hlook1; [inversion Hlookup1; subst |].
+        -- (*Now know x in fv p1 and y is in fv p2, so x is in a1*)
+          assert (Hmemx: aset_mem x (pat_fv p1)) by (eapply (a_equiv_p_vars Halphap); eauto).
+          rewrite <- (match_val_single_fv _ _ _ _ _ _ _ _ Hmatch1) in Hmemx.
+          rewrite <- amap_mem_keys, amap_mem_spec in Hmemx. unfold vsymbol in *.
+          destruct (amap_lookup a1 x) as [s1|] eqn : Hlookupa; [|discriminate].
+          (*Now use pattern match relation*)
+          assert (Hlookupb : amap_lookup a2 y = Some s1) by (rewrite <- Hopt; eauto).
+          rewrite !extend_val_lookup with (t:=s1) by auto.
+           (*Remove final cast*)
+          destruct x as [n1 x1]; destruct y as [n2 x2]; simpl in *; subst. 
+          unfold dom_cast; simpl.
+          (*Use typing result*)
+          pose proof (match_val_single_typs _ _ _ _ _ _ _ _ _ Hmatch1 _ _ Hlookupa) as Hsorteq. simpl in Hsorteq.
+          destruct (sort_eq_dec (v_subst vt x2) (projT1 s1)); auto.
+          exfalso; apply n; symmetry; assumption.
+        -- (*Second case*)
+          destruct (amap_lookup pm2 y) as [x1|] eqn : Hlook2; [inversion Hlookup2; subst |].
+          ++ (*Contradicts bijection*)
+            unfold bij_map in Hbij. rewrite <- Hbij in Hlook2. 
+            simpl in Hlook2; rewrite Hlook2 in Hlook1; discriminate.
+          ++ (*Both None, use Hval2, need to prove fv*)
+            rewrite !extend_val_notin; auto; rewrite amap_mem_keys_false;
+            [ rewrite (match_val_single_fv _ _ _ _ _ _ _ _ Hmatch2) |
+              rewrite (match_val_single_fv _ _ _ _ _ _ _ _ Hmatch1)];
+            intros C.
+            (*We need the other direction: every free variable in a pattern is in the resulting map*)
+            
+            ** (*Again use fv*)
+              , .
+
+
+
+ auto. destruct x as [n1 x1]; destruct y as [n2 x2]; simpl in *; subst. 
+              unfold dom_cast; simpl. apply Hvals2.
+              
+
+ auto.
+
+ try rewrite amap_mem_spec.
+
+
+ [| rewrite Hlookup1 | rewrite Hlook2]. Search amap_mem false amap_lookup. 
+            destruct (amap_lookup pm2 y) as [z|] eqn : Hget; auto; rewrite <- Hbij in Hget.
+            simpl in Hget. unfold vsymbol in *. rewrite Hget in Hlook1.
+
+ reflexivity.
+          eapply H; eauto.
+
+ 2: { 
+
+
+assert (Hlook2: amap_lookup pm2 y = Some x) by (apply Hbij; auto).
+          rewrite Hlook2 in Hlookup2.
+          Check extend_val_lookup.
+          Search extend_val_with_list amap_lookup.
+            apply Hbij. auto.
+
+        destruct Hlookup1 as [[Hxeq Hyeq] | [Hneq Hlookup1]];
+        destruct Hlookup2 as [[Hxeq2 Hyeq2] | [Hneq2 Hlookup2]]; subst; try contradiction.
+        * unfold substi. vsym_eq x x. vsym_eq y y.
+          (*Now use first IH*)
+          assert (e = eq_refl) by (apply UIP_dec, vsymbol_eq_dec).
+          assert (e0 = eq_refl) by (apply UIP_dec, vsymbol_eq_dec).
+          subst. simpl.
+          (*Remove final cast*)
+          destruct x as [n1 ty1]; destruct y as [n2 ty2]; simpl in *; subst.
+          assert (Heq = eq_refl) by (apply UIP_dec, vty_eq_dec). subst; unfold dom_cast; simpl.
+          eapply H; eauto.
+        * (*2nd case, easy*)
+          unfold substi. vsym_eq x x1. vsym_eq y x2.
+
+    + (*IH case*)
+      inversion Hps; subst; eauto.
+      erewrite <- IHps1; eauto. rewrite (Htm tm2 m1 m2 v1 v2 _ Hty1 Hty2) by auto. reflexivity.
+  -
+
+ assert (Hbij: bij_map pm1 pm2). {
+          apply a_equiv_p_bij in Halphap; auto.
+        
+
+
+Corollary a_equiv_p_bij {p1 p2: pattern} {res}:
+  a_equiv_p p1 p2 = Some res ->
+  bij_map (fst res) (snd res).
+Proof.
+  intros Halpha.
+  eapply alpha_equiv_p_bij; eauto.
+  apply bij_empty.
+Qed.
+
+(*Idea: for every binding (x, y) in first map, we know that x in fv of p1 and y in fv in p2*)
+Corollary a_equiv_p_vars {p1 p2: pattern} {res}
+  (Halpha: a_equiv_p p1 p2 = Some res) x y (Hmem: amap_lookup (fst res) x = Some y):
+  aset_mem x (pat_fv p1) /\ aset_mem y (pat_fv p2).
+Proof.
+  eapply alpha_equiv_p_vars in Hmem; eauto.
+  simpl in Hmem. rewrite amap_empty_get in Hmem. destruct_all; auto; discriminate.
+Qed.
+      
+
+
+      rewrite <- (Htm tm2 m1 m2 v1 v2 _ Hty1 Hty2) by auto. apply IHps1.
+
+
+
+
+match_val_single_alpha_p_full {ty: vty} {p1 p2: pattern}
+  (Hty1: pattern_has_type gamma p1 ty)
+  (Hty2: pattern_has_type gamma p2 ty)
+  (d: domain (dom_aux pd) (v_subst vt ty))
+  {res}
+  (Halpha: a_equiv_p p1 p2 = Some res):
+  opt_related (fun s1 s2 =>
+    forall x y t,
+    amap_lookup (fst res) x = Some y ->
+    amap_lookup s1 x = Some t <-> amap_lookup s2 y = Some t)
+  (match_val_single gamma_valid pd pdf vt ty p1 Hty1 d)
+  (match_val_single gamma_valid pd pdf vt ty p2 Hty2 d).
+
+
+    destruct (alpha_equiv_p (amap_empty, amap_empty)
+
+
+    + auto.
+
+
+ simpl; intros; destruct ps2; inversion Hps; auto.
+    destruct a as [p1 t1]. simpl.
+    destruct p as [p2 t2]. simpl.
+    rewrite <- (H _ _ v1 v2 _ Hty1 Hty2 Htm) at 1; auto.
+    
+    (*Now need to know [match_val_single] is same - separate lemmas*)
+    destruct ( match_val_single gamma_valid pd pdf vt tys2 p1 (Forall_inv Hpat1)
+    (term_rep v1 tm tys2 Hty1)) eqn : Hmatch1.
+    + (*In Some case, need to know how lists relate*)
+
+      (*First, get some info we need*)
+      assert (Hpeq: alpha_equiv_p (combine (pat_fv p1) (pat_fv p2)) p1 p2). {
+        specialize (Hall 0 ltac:(lia)); simpl in Hall.
+        bool_hyps; auto.
+      }
+      pose proof (alpha_equiv_p_fv_len_full _ _ Hpeq) as Hlen2.
+      destruct (  match_val_single gamma_valid pd pdf vt tys2 p2 (Forall_inv Hpat2)
+      (term_rep v1 tm tys2 Hty1)) eqn : Hmatch2.
+      * assert (A:=Hall). specialize (A 0 ltac:(lia)); simpl in A.
+        bool_hyps. rename H1 into Hp; rename H3 into Ht12.
+        inversion H0; subst. eapply H4. apply Ht12.
+        -- intros. 
+          unfold add_vals in H1.
+          rewrite in_firstb_app in H1.
+          bool_hyps; destruct H1 as [Hinfv | H1]; bool_hyps.
+          ++ (*Case 1: (x, y) are in free vars of p0 and p respectively.
+            Then we use [match_val_single_alpha_p_some] and
+            [match_val_single_nodup] to show that their valuations
+            are the same.*)
+            apply in_firstb_in in Hinfv.
+            assert (Hincom:=Hinfv).
+            rewrite in_combine_iff in Hinfv; wf_tac.
+            destruct Hinfv as [i [Hi Hith]].
+            specialize (Hith vs_d vs_d). inversion Hith.
+            (*Now, we know that x is in l by 
+              [match_val_single_free_var]*)
+            assert (Hinxl: In x (map fst l)). {
+              apply (match_val_single_free_var _ _ _ _ _ _ _ _ _ x) in Hmatch1.
+              auto.
+              apply Hmatch1. subst. wf_tac.
+            }
+            rewrite in_map_iff in Hinxl. destruct Hinxl as [bnd [Hx Hinbnd]].
+            destruct bnd as [x' t']. simpl in Hx. subst x'.
+            (*Now, we use [match_val_single_alpha_p_some] to show
+              that (y, t') is in l0*)
+            assert (Hinyl: In (y, t') l0). {
+              eapply match_val_single_alpha_p_some in Hmatch2.
+              rewrite <- Hmatch2. apply Hinbnd. apply Hp.
+              all: wf_tac. apply Hmatch1. 
+            }
+            (*Finally, we use NoDup of l, l0 
+              (from [match_val_single_nodup]) to give the binding*)
+            assert (Hnodup1: NoDup (map fst l)). {
+              eapply match_val_single_nodup in Hmatch1.
+              apply Hmatch1.
+            }
+            assert (Hnodup2: NoDup (map fst l0)). {
+              eapply match_val_single_nodup in Hmatch2.
+              apply Hmatch2.
+            }
+            rewrite !extend_val_lookup with(t:=t'); auto.
+            (*Now handle all the casting*)
+            destruct (sort_eq_dec (v_subst vt (snd x)) (projT1 t')).
+            ** destruct (sort_eq_dec (v_subst vt (snd y)) (projT1 t')).
+              {
+                destruct x; destruct y; simpl in *; subst.
+                destruct t'; simpl in *; subst; simpl.
+                assert (e0 = eq_refl). apply UIP_dec. apply sort_eq_dec.
+                rewrite H1. reflexivity. 
+              }
+              { 
+                exfalso.
+                rewrite Heq in e. contradiction.
+              }
+            ** (*contradiction case - types match in output
+              by [match_val_single_typs]*)
+              apply match_val_single_typs with(x:=x)(t:=t') in Hmatch1;
+              auto. exfalso. rewrite Hmatch1 in n. contradiction.
+              (*And we are done!*)
+          ++ (*Now in the other case, neither are free vars, so
+            we use Hvals2*)
+            repeat simpl_sumbool.
+            rewrite map_fst_combine in n0; wf_tac.
+            rewrite map_snd_combine in n; wf_tac.
+            assert (Hxl: ~ In x (map fst l)). {
+              intro C. 
+              apply match_val_single_free_var with(x:=x) in Hmatch1;
+              auto.
+              apply Hmatch1 in C. contradiction.
+            }
+            assert (Hyl0: ~ In y (map fst l0)). {
+              intro C.
+              apply match_val_single_free_var with(x:=y)in Hmatch2;
+              auto.
+              apply Hmatch2 in C; contradiction.
+            }
+            rewrite !extend_val_notin; wf_tac.
+        -- (*Here, we must show preservation of [Hvals2]*) 
+          unfold add_vals.
+          intros x. rewrite !map_app, !in_app_iff;
+          intros [Hnotx1 Hnotx2].
+          not_or Hnotx. rewrite map_fst_combine in Hnotx2; wf_tac.
+          rewrite map_snd_combine in Hnotx; wf_tac.
+          rewrite !extend_val_notin; wf_tac;
+          intro C.
+          ++ apply match_val_single_free_var with(x:=x) in Hmatch2;
+            auto.
+            apply Hmatch2 in C; contradiction.
+          ++ apply match_val_single_free_var with(x:=x) in Hmatch1;
+            auto.
+            apply Hmatch1 in C; contradiction.
+      * (*Contradiction: both are Some or both are None*)
+        exfalso.
+        rewrite <- match_val_single_alpha_p_none_iff in Hmatch2.
+        rewrite Hmatch2 in Hmatch1. inversion Hmatch1. apply Hpeq.
+    + (*In None case, both None, use IH*) 
+      assert (match_val_single gamma_valid pd pdf vt tys2 p2 (Forall_inv Hpat2)
+      (term_rep v1 tm tys2 Hty1)
+      = None). {
+        eapply match_val_single_alpha_p_none. 2: apply Hmatch1.
+        specialize (Hall 0 ltac:(lia)). simpl in Hall.
+        bool_hyps; auto. apply H1.
+      }
+      rewrite H1. apply IHps; auto; clear IHps.
+      * inversion H0; subst; auto.
+      * intros j Hj; specialize (Hall (S j) ltac:(lia)); simpl in Hall;
+        auto.
+    
+
+
+    generalize dependent ps2.
+    
+    induction ps; simpl; intros; destruct ps2; inversion Hps; auto.
+    destruct a as [p1 t1]. simpl.
+    destruct p as [p2 t2]. simpl.
+    rewrite <- (H _ _ v1 v2 _ Hty1 Hty2 Htm) at 1; auto.
+
+
+ rename H1 into Htm; rename H4 into Hps; rename H2 into Hall.
+    apply Nat.eqb_eq in Hps.
+    rewrite fold_is_true in Hall.
+    rewrite all2_forall with(d1:=(Pwild, tm_d))(d2:=(Pwild, tm_d)) in Hall; auto.
+    simpl_rep_full.
+    (*Need nested induction here*)
+    iter_match_gen Hty Htm1 Hpat1 Hty1.
+    iter_match_gen Hty2 Htm2 Hpat2 Hty2.
+    generalize dependent tys2.
+    generalize dependent ps2.
+
+
+
+    rewrite andb_true in Heq. destruct Heq as [Heq Hall].
+    rewrite andb_true in Heq.
+    
+
+
+    erewrite H, H0, H1; try reflexivity. erewr
+ erewrite H, H0, H1; eauto.
+      
+
+ erewrite H.
+      Search amap_lookup "impl".
+      destruct x1 as [n1 ty1]; destruct x2 as [n2 ty2]; simpl in Htyeq; subst. simpl.
+      unfold substi.
+      unfold substi
+       
+      erewrite H; eauto. apply Hvals.
+
+    
+
+ intros; eauto.
+    intros. rewrite Forall_forall in H. 
+    apply H with(vars:=vars); wf_tac.
+ 
+
+ contradiction.
+    destruct c0; simpl_rep_full.
+
+ simpl_rep_full.
+
 
 
 
